rustdemo/LinkedListSafe.v
@@ -9,11 +9,71 @@ Require Import Cop RustOp.
 Require Import Ctypes Rusttypes Rustlight.
 Require Import LinkedList.
 Require Import Values Globalenvs Memory.
+Require Import InitDomain.
+Require Import Events.
 Require Import Smallstep Rustlightown SmallstepLinkingSafe.
-
 
 Local Open Scope error_monad_scope.
 Import ListNotations.
+
+(* starN inside a function *)
+Fixpoint num_frames_cont (k: cont) : nat :=
+  match k with
+  | Kstop => O
+  | Kcall _ _ _ _ k' =>
+      S (num_frames_cont k')
+  | Kseq _ k
+  | Kloop _ k
+  | Kdropinsert _ _ k
+  | Kdropplace _ _ _ _ _ k
+  | Kdropcall _ _ _ _ k
+  | Klet _ _ k => num_frames_cont k
+  end.
+
+Definition num_frames (s: state) : nat :=
+  match s with
+  | State _ _ k _ _ _
+  | Callstate _ _ k _
+  | Returnstate _ k _
+  | Dropinsert _ _ _ k _ _ _
+  | Dropplace _ _ _ k _ _ _
+  | Dropstate _ _ _ _ k _ => num_frames_cont k
+  end.
+              
+
+
+Section CLOSURES.
+
+Context {genv: Type}.
+Context {state: Type}.
+
+Variable step: genv -> state -> trace -> state -> Prop.
+Variable numf: state -> nat.
+
+Inductive starNf (ge: genv): nat -> state -> trace -> state -> Prop :=
+  | starNf_refl: forall s,
+      starNf ge O s E0 s
+  | starNf_step: forall n s t t1 s' t2 s''
+      (STEP: step ge s t1 s')
+      (STAR: starNf ge n s' t2 s'')
+      (TRACE: t = t1 ** t2)
+      (FEQ: numf s = numf s'),
+      starNf ge (S n) s t s''.
+
+Remark starNf_star:
+  forall ge n s t s', starNf ge n s t s' -> star step ge s t s'.
+Proof.
+  induction 1; econstructor; eauto.
+Qed.
+
+Remark starNf_step_right ge: forall n s t t1 s' t2 s'',
+    starNf ge n s t1 s' -> step ge s' t2 s'' -> t = t1 ** t2 ->
+    numf s' = numf s'' ->
+    starNf ge (S n) s t s''.
+Admitted.
+
+End CLOSURES.
+
 
 Definition linked_list_sem := semantics linked_list_mod.
 
@@ -22,6 +82,11 @@ Section SOUNDNESS.
 Context (se : Genv.symtbl).
 
 Let ge := globalenv se linked_list_mod.
+
+Hypothesis wf_senv: forall id,
+    if in_dec ident_eq id (prog_defs_names linked_list_mod) then
+      exists b, Genv.find_symbol se id = Some b
+    else True.
 
 Inductive sound_find_cont : cont -> Prop :=
 | sound_find_Kstop:
@@ -44,6 +109,7 @@ Definition length_of_args (f: ident) : nat :=
 
 Inductive call_func (f: ident) : state -> Prop :=
 | call_func_intro: forall b vl k m
+    (* ensured by valid_query *)
     (SYM: Genv.invert_symbol se b = Some f)
     (** TODO: some property of k *)
     (SCONT: sound_cont f k)
@@ -75,44 +141,20 @@ Inductive return_find : state -> Prop :=
     return_find (Returnstate v k m).
 
 
-Fixpoint num_frames_cont (k: cont) : nat :=
-  match k with
-  | Kstop => O
-  | Kcall _ _ _ _ k' =>
-      S (num_frames_cont k')
-  | Kseq _ k
-  | Kloop _ k
-  | Kdropinsert _ _ k
-  | Kdropplace _ _ _ _ _ k
-  | Kdropcall _ _ _ _ k
-  | Klet _ _ k => num_frames_cont k
-  end.
-
-Definition num_frames (s: state) : nat :=
-  match s with
-  | State _ _ k _ _ _
-  | Callstate _ _ k _
-  | Returnstate _ k _
-  | Dropinsert _ _ _ k _ _ _
-  | Dropplace _ _ _ k _ _ _
-  | Dropstate _ _ _ _ k _ => num_frames_cont k
-  end.
-              
 
 Inductive sound_state : state -> Prop :=
 | find_state_internal1: forall s0 s1 t n
     (CALL: call_func find s0)
-    (STAR: starN step ge n s0 t s1)
-    (RAN: (0 <= n <= 20)%nat)
-    (* all execution is inside the current function *)
-    (NUMF: num_frames s0 = num_frames s1),
+    (STAR: starNf step num_frames ge n s0 t s1)
+    (RAN: (0 <= n <= 20)%nat),
     sound_state s1
 | find_state_internal2: forall s0 s1 t n,
     return_find s0 ->
-    starN step ge n s0 t s1 ->
-    (0 <= n <= 10)%nat ->  
-    num_frames s0 = num_frames s1 ->
+    starNf step num_frames ge n s0 t s1 ->
+    (0 <= n <= 10)%nat ->
     sound_state s1
+(* | find_state_call_process: forall , *)
+(*     sound_state (Callstate v al  *)
 | find_returnstate: forall v k m,
     sound_find_cont k ->
     sound_state (Returnstate v k m).
@@ -142,8 +184,8 @@ Lemma init_own_env_find_progress:
   generalize flag at 1 3.
   intros flag0 E. destruct flag0; try congruence.
   eexists; eauto.
-  unfold flag in E. unfold initParams, empty_map in *.
-  unfold collect_func in A.
+  unfold flag in E. unfold initParams, empty_map in *.  
+  unfold collect_func in A. 
   replace t with ((collect_stmt (Smallstep.globalenv (linked_list_sem se))
            (fn_body find_func)
            (fold_right
@@ -153,68 +195,7 @@ Lemma init_own_env_find_progress:
               (map
                  (fun elt : ident * type => Plocal (fst elt) (snd elt))
                  (fn_params find_func ++ fn_vars find_func))))) in *.
-  replace (check_own_env_consistency
-        (PTree.map
-           (fun (_ : positive) (_ : InitDomain.LPaths.t) =>
-            InitDomain.Paths.empty)
-           (collect_stmt (Smallstep.globalenv (linked_list_sem se))
-              (fn_body find_func)
-              (fold_right
-                 (InitDomain.collect_place
-                    (Smallstep.globalenv (linked_list_sem se)))
-                 (PTree.empty InitDomain.LPaths.t)
-                 (map
-                    (fun elt : ident * type =>
-                     Plocal (fst elt) (snd elt))
-                    (fn_params find_func ++ fn_vars find_func)))))
-        (PTree.map
-           (fun (_ : positive) (_ : InitDomain.LPaths.t) =>
-            InitDomain.Paths.empty)
-           (collect_stmt (Smallstep.globalenv (linked_list_sem se))
-              (fn_body find_func)
-              (fold_right
-                 (InitDomain.collect_place
-                    (Smallstep.globalenv (linked_list_sem se)))
-                 (PTree.empty InitDomain.LPaths.t)
-                 (map
-                    (fun elt : ident * type =>
-                     Plocal (fst elt) (snd elt))
-                    (fn_params find_func ++ fn_vars find_func)))))
-        (InitDomain.add_place_list
-           (collect_stmt (Smallstep.globalenv (linked_list_sem se))
-              (fn_body find_func)
-              (fold_right
-                 (InitDomain.collect_place
-                    (Smallstep.globalenv (linked_list_sem se)))
-                 (PTree.empty InitDomain.LPaths.t)
-                 (map
-                    (fun elt : ident * type =>
-                     Plocal (fst elt) (snd elt))
-                    (fn_params find_func ++ fn_vars find_func))))
-           (places_of_locals (fn_params find_func ++ fn_vars find_func))
-           (PTree.map
-              (fun (_ : positive) (_ : InitDomain.LPaths.t) =>
-               InitDomain.Paths.empty)
-              (collect_stmt (Smallstep.globalenv (linked_list_sem se))
-                 (fn_body find_func)
-                 (fold_right
-                    (InitDomain.collect_place
-                       (Smallstep.globalenv (linked_list_sem se)))
-                    (PTree.empty InitDomain.LPaths.t)
-                    (map
-                       (fun elt : ident * type =>
-                        Plocal (fst elt) (snd elt))
-                       (fn_params find_func ++ fn_vars find_func))))))
-        (collect_stmt (Smallstep.globalenv (linked_list_sem se))
-           (fn_body find_func)
-           (fold_right
-              (InitDomain.collect_place
-                 (Smallstep.globalenv (linked_list_sem se)))
-              (PTree.empty InitDomain.LPaths.t)
-              (map
-                 (fun elt : ident * type => Plocal (fst elt) (snd elt))
-                 (fn_params find_func ++ fn_vars find_func))))) with true in *. congruence.
-  reflexivity.
+  vm_compute in E. congruence.
   congruence.
   unfold collect_func in A. congruence.
 Qed.
@@ -241,6 +222,55 @@ Definition val_is_int (v: val) : bool :=
   | _ => false
   end.
 
+Lemma sound_cont_no_vars: forall f k,
+    sound_cont f k ->
+    cont_vars k = nil.
+Proof.
+  intros. unfold sound_cont in H. destruct ident_eq in H; try contradiction.
+  inv H; reflexivity.
+Qed.
+
+Lemma split_drop_place_find_retv: forall w,
+    collect_func ge find_func = OK w ->
+    split_drop_place ge (PathsMap.get _retv w) (Plocal _retv List_box) List_box = OK [(Plocal _retv List_box, true)].
+Proof using se.
+  intros. unfold collect_func in H.
+  vm_compute in H. inv H. reflexivity.
+Qed.
+
+Lemma split_drop_place_find_l: forall w,
+    collect_func ge find_func = OK w ->
+    split_drop_place ge (PathsMap.get l w) (Plocal l List_box) List_box = OK [(Pderef (Plocal l List_box) List_ty, true); (Plocal l List_box, false)].
+Proof using se.
+  intros. unfold collect_func in H.
+  vm_compute in H. inv H. reflexivity.
+Qed.
+
+Lemma split_drop_place_find_node: forall w,
+    collect_func ge find_func = OK w ->
+    split_drop_place ge (PathsMap.get node w) (Plocal node Node_ty) Node_ty = OK [(Pfield (Plocal node Node_ty) key type_int32s, true);
+    (Pfield (Plocal node Node_ty) LinkedList.val type_int32s, true);
+    (Pfield (Plocal node Node_ty) next List_box, true)].
+Proof using se.
+  intros. unfold collect_func in H.
+  vm_compute in H. inv H. reflexivity.  
+Qed.
+
+
+Lemma sound_call_cont_find: forall k,
+    sound_cont find k ->
+    (* Actually ck is the same as k *)
+    exists ck, call_cont k = Some ck
+          /\ sound_cont find ck.
+Admitted.
+
+Lemma call_cont_num_frames_eq: forall k1 k2,
+    call_cont k1 = Some k2 ->
+    num_frames_cont k1 = num_frames_cont k2.
+Proof.
+  induction k1; intros k2 CK; simpl in *; inv CK; auto.
+Qed.
+
 Lemma step_preservation_progress: forall s,
     sound_state s ->
     (not_stuck (linked_list_sem se) s \/ step_mem_error ge s)
@@ -266,10 +296,10 @@ Proof.
         do 2 eexists.
         econstructor; eauto.
       - intros. eapply find_state_internal1 with (n:= 1%nat); eauto.
-        econstructor; eauto. econstructor. lia.
-        inv H; simpl; auto. }
+        econstructor; eauto. econstructor. 
+        inv H; simpl; auto. lia. }
     (** take one step *)
-    inv H; try congruence.
+    inv STEP; try congruence.
     rewrite FIND in FIND0. inv FIND0.    
     unfold init_own_env in INITOWN.
     (* construct own_env *)
@@ -286,9 +316,8 @@ Proof.
     generalize flag at 1 3.
     intros flag0 E. destruct flag0; try congruence. intros. inv INITOWN.
     (* construct e *)
-    inv ENTRY. inv ALLOC. inv H8. inv H10. inv H11. inv H12. inv H13.
-    inv H14. inv H15. inv H16. inv H17.
-    inv H0.
+    inv ENTRY. inv ALLOC. inv H7. inv H9. inv H10. inv H11.
+    inv STAR0.
     (* stop here: evaluate the if statement *)
     { split.
       - left. red.
@@ -298,7 +327,7 @@ Proof.
           (* we should show thata v1 must be a pointer *)
           destruct (val_is_ptr v1) eqn: VPTR.
           * destruct v1; simpl in VPTR; try congruence.
-            destruct (Mem.valid_access_dec m' Mint32 b9 (Ptrofs.unsigned i) Readable) eqn: VA2.
+            destruct (Mem.valid_access_dec m' Mint32 b4 (Ptrofs.unsigned i) Readable) eqn: VA2.
             -- exploit Mem.valid_access_load. eapply v0. intros (v2 & LOAD2).
                destruct (val_is_int v2) eqn: VINT.
                ++ destruct v2; simpl in VINT; try congruence.
@@ -306,14 +335,16 @@ Proof.
                   
                   do 2 eexists.
                   (* evaluate if then else *)
-                  econstructor. econstructor. econstructor. econstructor.
+                  econstructor. econstructor. econstructor.
                   econstructor.
-                  do 8 (try rewrite PTree.gso; try (cbv delta; congruence)).
-                  rewrite PTree.gss. reflexivity.
-                  econstructor. simpl. eauto.
-                  eauto. eauto. simpl. unfold List_ty. eauto.
-                  simpl. reflexivity. reflexivity.
-                  reflexivity.
+                  econstructor.
+                  reflexivity. 
+                  econstructor. reflexivity.
+                  eauto. eauto. 1-3: reflexivity. 
+                  (** TODO: range check. Make it a memory error state *)
+                  simpl. unfold list_length_z. simpl.
+                  admit.
+                  reflexivity. 
                   simpl.
                   instantiate (1 := Int.eq i0 (Int.repr 0)).
                   destruct (Int.eq i0 (Int.repr 0)) eqn: EQZ; reflexivity.
@@ -327,163 +358,615 @@ Proof.
         + admit.
       (* Invariant preservation *)
       - intros. eapply find_state_internal1 with (n:=2%nat); eauto.
-        eapply starN_step_right; eauto. lia.
-        inv H; simpl; auto. }
+        eapply starNf_step_right; eauto.
+        inv H; simpl; auto. lia. }
     (* destruct the if step *)
-    inv H.
-    2: { destruct H18; unfold find_body in *; try congruence. }
+    inv STEP.
+    2: { destruct H11; unfold find_body in *; try congruence. }
     (* get the bool value *)
-    simpl in H22. inv H20. inv H0.
-    simpl in H5. unfold List_ty in H5. inv H5. simpl in H6.
-    rewrite PTree.gss in H6. inv H6. simpl in H17.
-    vm_compute in H17. inv H17.
-    destruct (Int.eq tag (Int.repr 0)) eqn: EQZ; vm_compute in H22; inv H22.
+    simpl in H15. inv H13. inv H0.
+    simpl in PTY. unfold List_ty in PTY. inv PTY.
+    vm_compute in CO. inv CO. vm_compute in FTAG. inv FTAG.
+    simpl in RANGE. unfold list_length_z in RANGE. simpl in RANGE.
+    destruct (Int.eq tag (Int.repr 0)) eqn: EQZ; vm_compute in H15; inv H15.
     (** evaluate the if branch *)
-    { inv H1.
+    { inv STAR; cbn [num_frames] in *.
+      (* stop here: evaluate Ssequence *)
+      { split.
+        - left. red. do 2 right.
+          do 2 eexists. econstructor.
+        - intros. eapply find_state_internal1 with (n:=3%nat); eauto.
+          eapply starNf_step_right; eauto. 
+          inv H; simpl; auto. lia. }
+      inv STEP.
+      2: { destruct H11; congruence. }
+      inv STAR0; cbn [num_frames num_frames_cont] in *.
+      (* stop here: evaluate Sassign to Dassign *)
+      { split.
+        - left. red. do 2 right.
+          do 2 eexists. econstructor.
+        - intros. eapply find_state_internal1 with (n:=4%nat); eauto.
+          eapply starNf_step_right; eauto. 
+          inv H; simpl; auto. lia. }
+      inv STEP. inv STAR; cbn [num_frames num_frames_cont] in *.
+      (* stop here: evaluate step_dropinsert_to_dropplace_reassign *)
+      { split.
+        - left. red. do 2 right.
+          do 2 eexists. econstructor.
+          eapply step_dropinsert_to_dropplace_reassign; auto.
+          unfold init_place. cbn [own_universe].
+          eapply split_drop_place_find_retv; eauto.
+        - intros. eapply find_state_internal1 with (n:=5%nat); eauto.
+          eapply starNf_step_right; eauto. 
+          inv H; inv SDROP; simpl; auto. lia. }
+      inv STEP. inv SDROP; vm_compute in OWNTY; try congruence.
+      erewrite split_drop_place_find_retv in SPLIT; eauto. inv SPLIT.
+      inv STAR0; cbn [num_frames num_frames_cont] in *.
+      (* stop here: evaluate step_dropplace_init1 *)
+      { split.
+        - left. red. do 2 right.
+          do 2 eexists. econstructor.
+          eapply step_dropplace_init1.
+          unfold is_init, init_place. simpl.
+          unfold collect_func in A. vm_compute in A. inv A. 
+          reflexivity.
+        - intros. eapply find_state_internal1 with (n:=6%nat); eauto.
+          eapply starNf_step_right; eauto.
+          inv H; inv SDROP; simpl; auto. lia. }
+      inv STEP. inv SDROP.
+      2: { unfold is_init, init_place in OWN. simpl in OWN.
+           unfold collect_func in A. vm_compute in A. inv A.
+           vm_compute in OWN. congruence. }
+      2: { simpl in SCALAR. congruence. }
+      clear NOTOWN.
+      inv STAR; cbn [num_frames num_frames_cont] in *.
+      (* stop here: evaluate step_dropplace_return *)
+      { split.
+        - left. red. do 2 right.
+          do 2 eexists. econstructor.
+          eapply step_dropplace_return.
+        - intros. eapply find_state_internal1 with (n:=7%nat); eauto.
+          eapply starNf_step_right; eauto. 
+          inv H; inv SDROP; simpl; auto. lia. }
+      inv STEP. inv SDROP.
+      inv STAR0; cbn [num_frames num_frames_cont] in *.
+      (* stop here: ealuate step_dropinsert_assign *)
+      { split.
+        - destruct (Mem.valid_access_dec m' Mptr b1 0 Readable) eqn: VA1.
+          (* The argument l is loadable *)
+          + exploit Mem.valid_access_load. eapply v. intros (?v & ?LOAD).
+            * destruct (sem_cast v0 List_box List_box) eqn: CAST1.
+              (* v0 can be casted *)
+              -- destruct (Mem.valid_access_dec m' Mptr b2 0 Writable) eqn: VA2.
+                 (* The return variable is writable *)
+                 ++ edestruct Mem.valid_access_store with (v:= v1) as (?m & ?STORE).
+                    eapply v2.
+                    left. red. do 2 right.
+                    do 2 eexists. econstructor.
+                    econstructor; eauto.
+                    simpl. unfold List_box. congruence.
+                    econstructor. reflexivity.
+                    econstructor. econstructor. econstructor.
+                    reflexivity. econstructor. reflexivity.
+                    eauto. econstructor. reflexivity. eauto.
+                 (* The return variable is not writable *)
+                 ++ right. econstructor.
+                    eapply step_dropinsert_assign_error3.
+                    econstructor. reflexivity.
+                    econstructor. econstructor. econstructor.
+                    reflexivity. econstructor. reflexivity.
+                    eauto. eauto.
+                    eapply assign_loc_value_mem_error. reflexivity.
+                    eauto.
+              (* v0 cannot be casted *)
+              -- admit.
+          (* The argument l is not loadable *)
+          + right. econstructor.
+            eapply step_dropinsert_assign_error1.
+            econstructor. eapply eval_Eplace_error2.
+            econstructor. reflexivity.
+            econstructor. reflexivity. eauto.
+        - intros. eapply find_state_internal1 with (n:=8%nat); eauto.
+          eapply starNf_step_right; eauto. 
+          inv H; inv SDROP; simpl; auto. lia. }
+      inv STEP. inv SDROP.
+      inv STAR; cbn [num_frames num_frames_cont] in *.
+      (* stop here: evaluate Kseq *)
+      { split.
+        - left. red. do 2 right.
+          do 2 eexists. econstructor.
+        - intros. eapply find_state_internal1 with (n:=9%nat); eauto.
+          eapply starNf_step_right; eauto. 
+          inv H; simpl; auto. lia. }
+      inv STEP.
+      inv STAR0; cbn [num_frames num_frames_cont] in *.
+      (* stop here: evaluate Sreturn *)
+      { split.
+        - left. red. do 2 right.
+          do 2 eexists. econstructor.
+        - intros. eapply find_state_internal1 with (n:=10%nat); eauto.
+          eapply starNf_step_right; eauto. 
+          inv H; simpl; auto. lia. }
+      inv STEP.
+      2: { destruct H11; congruence. }
+      inv STAR; cbn [num_frames num_frames_cont] in *.
+      (* evaluate step_dropinsert_return_before *)
+      { split.
+        - left. red. do 2 right.
+          do 2 eexists. econstructor.
+          erewrite sound_cont_no_vars; eauto.          
+          eapply step_dropinsert_return_before.
+        - intros. eapply find_state_internal1 with (n:=11%nat); eauto.
+          eapply starNf_step_right; eauto. 
+          inv H; inv SDROP; simpl; auto. lia. }
+      inv STEP.
+      erewrite sound_cont_no_vars in SDROP; eauto.
+      inv SDROP. destruct NOTRETURN; congruence.
+      inv STAR0; cbn [num_frames num_frames_cont] in *.
+      (* stop here: evaluate step_dropinsert_to_dropplace_return *)
+      { split.
+        - left. red. do 2 right.
+          do 2 eexists. econstructor.
+          eapply step_dropinsert_to_dropplace_return.
+          reflexivity. reflexivity.
+          eapply split_drop_place_find_l; eauto.
+        - intros. eapply find_state_internal1 with (n:=12%nat); eauto.
+          eapply starNf_step_right; eauto. 
+          inv H; inv SDROP; simpl; auto. lia. }
+      inv STEP. inv SDROP.
+      2: { unfold List_box in OWNTY0. vm_compute in OWNTY0. congruence. }
+      erewrite split_drop_place_find_l in SPLIT; eauto. inv SPLIT.
+      inv STAR; cbn [num_frames num_frames_cont] in *.
+      (* stop here: evaluate step_dropplace_init1 *)
+      { split.
+        - left. red. do 2 right.
+          do 2 eexists. econstructor.
+          eapply step_dropplace_init1.
+          unfold collect_func in A. vm_compute in A. inv A.
+          reflexivity.
+        - intros. eapply find_state_internal1 with (n:=13%nat); eauto.
+          eapply starNf_step_right; eauto. 
+          inv H; inv SDROP; simpl; auto. lia. }
+      inv STEP. inv SDROP.
+      2: { unfold collect_func in A. vm_compute in A. inv A.
+           vm_compute in OWN. congruence. }
+      2: { unfold collect_func in A. vm_compute in A. inv A.
+           vm_compute in OWN. congruence. }
+      clear NOTOWN. inv STAR0.
+      (* stop here: evaluate step_dropplace_init1 *)
+      { split.
+        - left. red. do 2 right.
+          do 2 eexists. econstructor.
+          eapply step_dropplace_init1.
+          unfold collect_func in A. vm_compute in A. inv A.
+          reflexivity.
+        - intros. eapply find_state_internal1 with (n:=14%nat); eauto.
+          eapply starNf_step_right; eauto. 
+          inv H; inv SDROP; simpl; auto. lia. }
+      inv STEP. inv SDROP.
+      2: { unfold collect_func in A. vm_compute in A. inv A.
+           vm_compute in OWN. congruence. }
+      2: { unfold collect_func in A. vm_compute in A. inv A.
+           vm_compute in OWN. congruence. }
+      clear NOTOWN.
+      inv STAR; cbn [num_frames num_frames_cont] in *.
+      (* stop here: evaluate step_dropplace_return *)
+      { split.
+        - left. red. do 2 right.
+          do 2 eexists. econstructor.
+          eapply step_dropplace_return.
+        - intros. eapply find_state_internal1 with (n:=15%nat); eauto.
+          eapply starNf_step_right; eauto. 
+          inv H; inv SDROP; simpl; auto. lia. }
+      inv STEP. inv SDROP.
+      inv STAR0; cbn [num_frames num_frames_cont] in *.
+      (* stop here: evaluate step_dropinsert_skip_return *)
+      { split.
+        - left. red. do 2 right.
+          do 2 eexists. econstructor.
+          eapply step_dropinsert_skip_return.
+          reflexivity.
+        - intros. eapply find_state_internal1 with (n:=16%nat); eauto.
+          eapply starNf_step_right; eauto. 
+          inv H; inv SDROP; simpl; auto. lia. }
+      inv STEP. inv SDROP.
+      vm_compute in OWNTY1. congruence.
+      inv STAR; cbn [num_frames num_frames_cont] in *.
+      (* stop here: evaluate step_dropinsert_return_after *)
+      { split.
+        - destruct (Mem.valid_access_dec m5 Mptr b2 0 Readable) eqn: ?VA.
+          + exploit Mem.valid_access_load. eapply v0.
+            intros (?v & ?LOAD).
+            destruct (sem_cast v2 List_box List_box) eqn: ?CAST.
+            * destruct (Mem.free_list m5 [(b3, 0, 16); (b1, 0, 8); (b2, 0, 8); (b0, 0, 4)]) eqn: ?FREELIST.
+              -- left. red. do 2 right.
+                 exploit sound_call_cont_find; eauto.
+                 intros (ck & CK & SCK).
+                 do 2 eexists. econstructor.
+                 eapply step_dropinsert_return_after.
+                 econstructor. econstructor. econstructor. reflexivity.
+                 econstructor. reflexivity. eauto.
+                 eauto. eauto. 
+                 instantiate (1 := [(b3, 0, 16); (b1, 0, 8); (b2, 0, 8); (b0, 0, 4)]).
+                 reflexivity. eauto.
+              (* free_list memory error *)
+              -- right. econstructor.
+                 eapply step_dropinsert_return_error2; eauto.
+            (* sem_cast fails *)
+            * admit.
+          + right. econstructor.
+            eapply step_dropinsert_return_error1; eauto.
+            econstructor. eapply eval_Eplace_error2.
+            econstructor. reflexivity.
+            econstructor. reflexivity. eauto.
+        - intros. inv H. inv SDROP.
+          exploit sound_call_cont_find; eauto.
+          intros (ck1 & CK & SCK). rewrite CONT in CK. inv CK.          
+          eapply find_returnstate. eauto. }
+      (* show that it cannot take more step using num_frames unchanged
+      property *)
+      inv STEP. inv SDROP.
+      inv STAR0; cbn [num_frames num_frames_cont] in *.
+      (** show that the returnstate can take a step *)
+      { exploit sound_call_cont_find; eauto.
+        intros (ck1 & CK & SCK). rewrite CONT in CK. inv CK.
+        vm_compute in SCK. inv SCK.
+        (* ck1 is Kstop *)
+        - split.
+          (* final state *)
+          + left. red. left.
+            eexists. econstructor.
+          + intros. inv H.
+        (** TODO: ck1 is Kcall. Fill this code after finishing calling
+        find *)
+        - admit. }
+      (* num frames contradiction *)
+      inv STEP.
+      simpl in FEQ16.
+      exfalso. eapply Nat.neq_succ_diag_l; eauto. }
+        
+    (* evaluate the else branch *)
+    { cbn [num_frames num_frames_cont] in *.
+      (* show that the tag is one *)
+      generalize (Int.unsigned_range tag). intros TAGPOS.
+      destruct (zeq (Int.unsigned tag) 0). rewrite <- e in EQZ.
+      rewrite Int.repr_unsigned in EQZ. rewrite Int.eq_true in EQZ. congruence.
+      assert (EQONE: Int.unsigned tag = 1). lia.
+      inv STAR; cbn [num_frames num_frames_cont] in *.
       (* stop here: evaluate Slet *)
       { split.
         - left. red. do 2 right.
           do 2 eexists. econstructor.
         - intros. eapply find_state_internal1 with (n:=3%nat); eauto.
-          eapply starN_step_right; eauto. lia.
-          inv H; simpl; auto. }
-      inv H.
-      2: { destruct H20; try congruence. }
-      inv H0.
-      (* stop here: evaluate ssequence *)
+          eapply starNf_step_right; eauto. 
+          inv H; simpl; auto. lia. }
+      inv STEP.
+      2: { destruct H11; congruence. }
+      inv STAR0; cbn [num_frames num_frames_cont] in *.
+      (* stop here: evaluate Ssequence *)
       { split.
         - left. red. do 2 right.
           do 2 eexists. econstructor.
         - intros. eapply find_state_internal1 with (n:=4%nat); eauto.
-          eapply starN_step_right; eauto. lia.
-          inv H; simpl; auto. }
-      inv H. inv H1.
-      (* stop here: evaluate to Dassign *)
+          eapply starNf_step_right; eauto. 
+          inv H; simpl; auto. lia. }
+      inv STEP.
+      inv STAR; cbn [num_frames num_frames_cont] in *.
+      (* stop here: evaluate Sassign to Dassign *)
       { split.
         - left. red. do 2 right.
           do 2 eexists. econstructor.
         - intros. eapply find_state_internal1 with (n:=5%nat); eauto.
-          eapply starN_step_right; eauto. lia.
-          inv H; simpl; auto. }
-      inv H. inv H0.
-      (* stop here: evaluate step_dropinsert_skip_reassign *)
+          eapply starNf_step_right; eauto. 
+          inv H; simpl; auto. lia. }
+      inv STEP.
+      inv STAR0; cbn [num_frames num_frames_cont] in *.
+      (* stop here: evaluate step_dropinsert_to_dropplace_reassign *)
       { split.
         - left. red. do 2 right.
           do 2 eexists. econstructor.
-          eapply step_dropinsert_skip_reassign; auto.
+          eapply step_dropinsert_to_dropplace_reassign; auto.
+          unfold init_place. cbn [own_universe].
+          eapply split_drop_place_find_node; eauto.
         - intros. eapply find_state_internal1 with (n:=6%nat); eauto.
-          eapply starN_step_right; eauto. lia.
-          inv H; inv SDROP; simpl; auto. }
-      inv H. inv SDROP; vm_compute in OWNTY; try congruence.
-      inv H1.
-      (* stop here: ealuate step_dropinsert_assign *)
+          eapply starNf_step_right; eauto. 
+          inv H; inv SDROP; simpl; auto. lia. }
+      inv STEP. inv SDROP; vm_compute in OWNTY; try congruence.
+      erewrite split_drop_place_find_node in SPLIT; eauto. inv SPLIT.
+      inv STAR; cbn [num_frames num_frames_cont] in *.
+      (* evaluate step_dropplace_init1 *)
       { split.
         - left. red. do 2 right.
           do 2 eexists. econstructor.
-          eapply step_dropinsert_assign; auto.
-          simpl. congruence.
-          econstructor. reflexivity.
-          (* evaluate *l *)
-          econstructor. econstructor. econstructor.
-          eauto. reflexivity. reflexivity. eauto.
-          replace tag with (Int.repr 0). reflexivity.
-          generalize (Int.eq_spec tag (Int.repr 0)). rewrite EQZ. auto.
-          simpl. instantiate (1 := 8). reflexivity.
-          econstructor. simpl. eauto.
-          Mem.load_cast
-          Int.eq_
+          eapply step_dropplace_init1.
+          unfold collect_func in A. vm_compute in A. inv A.
           reflexivity.
-          repeat econstructor. 
-        Lemma starN_step_r: forall genv step 
+        - intros. eapply find_state_internal1 with (n:=7%nat); eauto.
+          eapply starNf_step_right; eauto. 
+          inv H; inv SDROP; simpl; auto. lia. }
+      inv STEP. inv SDROP.
+      2: { unfold collect_func in A. vm_compute in A. inv A.
+           vm_compute in OWN. congruence. }
+      2: { unfold collect_func in A. vm_compute in A. inv A.
+           vm_compute in OWN. congruence. }
+      clear NOTOWN.
+      inv STAR0; cbn [num_frames num_frames_cont] in *.
+      (* evaluate step_dropplace_init1 *)
+      { split.
+        - left. red. do 2 right.
+          do 2 eexists. econstructor.
+          eapply step_dropplace_init1.
+          unfold collect_func in A. vm_compute in A. inv A.
+          reflexivity.
+        - intros. eapply find_state_internal1 with (n:=8%nat); eauto.
+          eapply starNf_step_right; eauto. 
+          inv H; inv SDROP; simpl; auto. lia. }
+      inv STEP. inv SDROP.
+      2: { unfold collect_func in A. vm_compute in A. inv A.
+           vm_compute in OWN. congruence. }
+      2: { unfold collect_func in A. vm_compute in A. inv A.
+           vm_compute in OWN. congruence. }
+      clear NOTOWN.
+      inv STAR; cbn [num_frames num_frames_cont] in *.
+      (* evaluate step_dropplace_init1 *)
+      { split.
+        - left. red. do 2 right.
+          do 2 eexists. econstructor.
+          eapply step_dropplace_init1.
+          unfold collect_func in A. vm_compute in A. inv A.
+          reflexivity.
+        - intros. eapply find_state_internal1 with (n:=9%nat); eauto.
+          eapply starNf_step_right; eauto. 
+          inv H; inv SDROP; simpl; auto. lia. }
+      inv STEP. inv SDROP.
+      2: { unfold collect_func in A. vm_compute in A. inv A.
+           vm_compute in OWN. congruence. }
+      2: { unfold collect_func in A. vm_compute in A. inv A.
+           vm_compute in OWN. congruence. }
+      clear NOTOWN.
+      inv STAR0; cbn [num_frames num_frames_cont] in *.
+      (* stop here: evaluate step_dropplace_return *)
+      { split.
+        - left. red. do 2 right.
+          do 2 eexists. econstructor.
+          eapply step_dropplace_return.
+        - intros. eapply find_state_internal1 with (n:=10%nat); eauto.
+          eapply starNf_step_right; eauto. 
+          inv H; inv SDROP; simpl; auto. lia. }
+      inv STEP. inv SDROP.
+      inv STAR; cbn [num_frames num_frames_cont] in *.      
+      (* stop here: evaluate step_dropinsert_assign *)
+      { split.
+        (* Note that the evaluation of conditional expression provides
+        the fact of loading *l *)        
+        - destruct (Mem.range_perm_dec m' b5 (Ptrofs.unsigned (Ptrofs.add ofs (Ptrofs.repr 8))) ((Ptrofs.unsigned (Ptrofs.add ofs (Ptrofs.repr 8))) + 16) Cur Readable).
+          + exploit Mem.range_perm_loadbytes. eapply r. intros (bys & LOADBYTES).
+            destruct (Mem.range_perm_dec m' b3 0 (0 + 16) Cur Writable).
+            * edestruct Mem.range_perm_storebytes with (bytes:= bys) as (?m & ?STOREBYTES).
+              erewrite Mem.loadbytes_length; eauto. eauto.
+              left. red. do 2 right.
+              do 2 eexists. econstructor.
+              econstructor; eauto.
+              vm_compute. congruence.
+              econstructor. reflexivity.
+              econstructor. econstructor. econstructor.
+              eauto. reflexivity. reflexivity. eauto.
+              rewrite EQONE. reflexivity.
+              instantiate (1 := 8). reflexivity.
+              eapply deref_loc_copy. eauto.
+              simpl. reflexivity.
+              (* assign_loc_copy *)
+              eapply do_assign_loc_sound.
+              unfold do_assign_loc.
+              replace (sizeof (Smallstep.globalenv (linked_list_sem se))
+               (typeof_place (Plocal node Node_ty))) with 16 by reflexivity.
+              rewrite LOADBYTES.
+              rewrite Ptrofs.unsigned_zero. rewrite STOREBYTES.
+              destruct check_assign_copy.
+              -- reflexivity.
+              (** TODO: we can treat check_assign_copy failure as a
+              kind of memory error which can be ruled out in move
+              checking. The approach is that we add a case of memory
+              error in step_assign when the type of LHS is
+              Tstruct/Tvariant. We also check the RHS must be (Eplace
+              p') so that we can prove check_assign_copy success by
+              case analysis of (RHS = p') or (RHS <> p'), using the
+              fact that different place must have different location
+              *)
+              -- admit.
+            * right. econstructor.
+              eapply step_dropinsert_assign_error3.
+              econstructor. reflexivity.
+              econstructor. econstructor. econstructor.
+              eauto. reflexivity. reflexivity. eauto.
+              rewrite EQONE. reflexivity.
+              instantiate (1 := 8). reflexivity.
+              eapply deref_loc_copy. eauto.
+              simpl. reflexivity.
+              eapply assign_loc_copy_mem_error2; eauto.
+          + right. econstructor.
+            eapply step_dropinsert_assign_error3.
+            econstructor. reflexivity.
+            econstructor. econstructor. econstructor.
+            eauto. reflexivity. reflexivity. eauto.
+            rewrite EQONE. reflexivity.
+            instantiate (1 := 8). reflexivity.
+            eapply deref_loc_copy. eauto.
+            simpl. reflexivity.
+            eapply assign_loc_copy_mem_error1; eauto.
+        - intros. eapply find_state_internal1 with (n:=11%nat); eauto.
+          eapply starNf_step_right; eauto. 
+          inv H; inv SDROP; simpl; auto. lia. }
+      inv STEP. inv SDROP.
+      inv STAR0; cbn [num_frames num_frames_cont] in *.
+      (* stop here: evaluate skip_seq *)
+      { split.
+        - left. red. do 2 right.
+          do 2 eexists. econstructor.
+        - intros. eapply find_state_internal1 with (n:=12%nat); eauto.
+          eapply starNf_step_right; eauto. 
+          inv H; simpl; auto. lia. }
+      inv STEP.
+      inv STAR; cbn [num_frames num_frames_cont] in *.
+      (* stop here: evaluate Ssequence *)
+      { split.
+        - left. red. do 2 right.
+          do 2 eexists. econstructor.
+        - intros. eapply find_state_internal1 with (n:=13%nat); eauto.
+          eapply starNf_step_right; eauto. 
+          inv H; simpl; auto. lia. }
+      inv STEP.
+      inv STAR0; cbn [num_frames num_frames_cont] in *.
+      (* evaluate Sifthenelse *)
+      { split.
+        - destruct (Mem.valid_access_dec m5 Mint32 b0 0 Readable).
+          + exploit Mem.valid_access_load. eauto.
+            intros (?v & ?LOAD).
+            destruct (sem_cast v2 type_int32s type_int32s) eqn: ?CAST.
+            * destruct (Mem.valid_access_dec m5 Mint32 b3 0 Readable).
+              -- exploit Mem.valid_access_load. eauto.
+                 intros (?v & ?LOAD).
+                 destruct (sem_cast v5 type_int32s type_int32s) eqn: ?CAST.
+                 ++ exploit cast_val_is_casted. eapply CAST. intros ?CASTED.
+                    exploit cast_val_is_casted. eapply CAST0. intros ?CASTED.
+                    inv CASTED. inv CASTED0.
+                    exploit sem_cast_id. eapply CAST. intros ?CCAST.
+                    exploit sem_cast_id. eapply CAST0. intros ?CCAST.
+                    left. red. do 2 right.
+                    do 2 eexists. econstructor.
+                    (* evaluate the binary equal *)
+                    econstructor. econstructor.
+                    econstructor. econstructor. reflexivity.
+                    econstructor. reflexivity. eauto.
+                    econstructor. econstructor. econstructor. reflexivity.
+                    reflexivity. reflexivity.
+                    reflexivity.
+                    econstructor. reflexivity. eauto.
+                    reflexivity. reflexivity.
+                    simpl. unfold sem_cmp, sem_binarith. simpl.
+                    erewrite CCAST. rewrite CCAST0.
+                    reflexivity. reflexivity. simpl.
+                    instantiate (1 := Int.eq n n1). 
+                    destruct (Int.eq n n1) eqn: ?IEQ; reflexivity.
+                 (* cast fails *)
+                 ++ admit.
+              (* load fails *)
+              -- right.
+                 eapply step_ifthenelse_error.
+                 econstructor. econstructor.
+                 right. eapply eval_Eplace_error2.
+                 econstructor. econstructor. reflexivity. reflexivity.
+                 econstructor. reflexivity.
+                 econstructor. reflexivity. eauto.
+            (* cast fails *)
+            *  admit.
+          (* load fails *)
+          + right.
+            eapply step_ifthenelse_error.
+            econstructor. econstructor.
+            left. eapply eval_Eplace_error2.
+            econstructor. econstructor. 
+            econstructor. reflexivity.
+            eauto.
+        - intros. eapply find_state_internal1 with (n:=14%nat); eauto.
+          eapply starNf_step_right; eauto. 
+          inv H; simpl; auto. lia. }
+      inv STEP.
+      destruct b6.
+      
+      (* evaluate the true branch *)
+      { inv STAR; cbn [num_frames num_frames_cont] in *.
+        (* evaluate Scall to Dcall *)
+        { split.
+          - left. red. do 2 right.
+            do 2 eexists. econstructor.
+          - intros. eapply find_state_internal1 with (n:=15%nat); eauto.
+            eapply starNf_step_right; eauto. 
+            inv H; simpl; auto. lia. }
+        inv STEP.
+        inv STAR0; cbn [num_frames num_frames_cont] in *.
+        (* evaluate step_dropinsert_skip_reassign *)
+        { split.
+          - left. red. do 2 right.
+            do 2 eexists. econstructor.
+            eapply step_dropinsert_skip_reassign.
+            reflexivity.
+          - intros. eapply find_state_internal1 with (n:=16%nat); eauto.
+            eapply starNf_step_right; eauto. 
+            inv H; inv SDROP; simpl; auto. lia.}
+        inv STEP. inv SDROP.
+        vm_compute in OWNTY0. congruence. clear OWNTY0.
+        inv STAR; cbn [num_frames num_frames_cont] in *.
+        (* evaluate Dcall *)
+        { split.
+          - destruct (Mem.valid_access_dec m5 Mint32 b3 4 Readable).
+            + exploit Mem.valid_access_load. eauto.
+              intros (?v & ?LOAD).
+              destruct (sem_cast v3 type_int32s type_int32s) eqn: ?CAST.
+              * left. red. do 2 right.
+                (* construct the block of process *)
+                generalize (wf_senv process). intros FINDPRO.
+                simpl in FINDPRO. destruct FINDPRO as (?b & FINDPRO).
+                do 2 eexists. econstructor. econstructor.
+                reflexivity. reflexivity.
+                econstructor. econstructor. eauto.
+                eapply deref_loc_reference. reflexivity.
+                (* evaluate the arguments *)
+                econstructor.
+                econstructor. econstructor. econstructor.
+                econstructor. reflexivity. reflexivity.
+                reflexivity. reflexivity. econstructor. reflexivity.
+                eauto. eauto.
+                econstructor.
+                (* find_funct *)
+                simpl. rewrite dec_eq_true. unfold Genv.find_funct_ptr.
+                rewrite Genv.find_def_spec.
+                erewrite Genv.find_invert_symbol; eauto.
+                reflexivity. reflexivity.
+                simpl. auto.
+              (* sem_cast fails *)
+              * admit.
+            (* load fails *)
+            + right.
+              generalize (wf_senv process). intros FINDPRO.
+              simpl in FINDPRO. destruct FINDPRO as (?b & FINDPRO).
+              econstructor.
+              eapply step_dropinsert_call_error2.   
+              econstructor. econstructor. eauto.
+              eapply deref_loc_reference. reflexivity.
+              reflexivity. econstructor. econstructor.
+              eapply eval_Eplace_error2. econstructor.
+              econstructor. reflexivity. reflexivity. reflexivity.
+              reflexivity. econstructor. reflexivity.
+              eauto.
+          - intros.
+            eapply 
+
+            (in_dec ident_eq process (prog_defs_names linked_list_mod)).
+            
+          simpl.
+          eapply do_assign_loc
+            econstructor. reflexivity.
+          econstructor. reflexivity.
+          eauto. reflexivity. reflexivity.
+                 
+          
+      Cop.val_casted
+      eval_Ebinop
+      destruct (Int.eq_
+        length
         
-        econstructor.
-        Mem.valid_access_load
-    
-        Lemma init_own_env_find_progress:
-          exists own, init_own_env (Smallstep.globalenv (linked_list_sem se)) find_func =
- OK own.
-        
-        2: { unfold init_own_env.
-             destruct collect_func eqn: A. cbn [bind].
-             set (empty_map := (PTree.map
-         (fun (_ : positive) (_ : InitDomain.LPaths.t) =>
-            InitDomain.Paths.empty) t)) in *.
-             set (initParams:= (InitDomain.add_place_list t
-         (places_of_locals (fn_params find_func ++ fn_vars find_func))
-         empty_map)) in *.
-             set (flag := check_own_env_consistency empty_map empty_map initParams t) in *.
-             generalize (eq_refl flag).             
-             generalize flag at 1 3.
-             intros flag0 E. destruct flag0; try congruence.
-             
-             generalize (check_own_env_consistency
-       (PTree.map
-          (fun (_ : positive) (_ : InitDomain.LPaths.t) =>
-           InitDomain.Paths.empty) t)
-       (PTree.map
-          (fun (_ : positive) (_ : InitDomain.LPaths.t) =>
-           InitDomain.Paths.empty) t)
-       (InitDomain.add_place_list t
-          (places_of_locals (fn_params find_func ++ fn_vars find_func))
-          (PTree.map
-             (fun (_ : positive) (_ : InitDomain.LPaths.t) =>
-              InitDomain.Paths.empty) t))) at 1,3 .
+      
+            simpl.
+            Mem.load_cast val_casted
+              val_casted
+              Int.eq_
+              reflexivity.
+            repeat econstructor.
+            Lemma starN_step_r: forall genv step
+Admitted.
 
-             
-             replace (check_own_env_consistency
-      (PTree.map
-         (fun (_ : positive) (_ : InitDomain.LPaths.t) =>
-          InitDomain.Paths.empty)
-         (collect_func (Smallstep.globalenv (linked_list_sem se))
-            find_func))
-      (PTree.map
-         (fun (_ : positive) (_ : InitDomain.LPaths.t) =>
-          InitDomain.Paths.empty)
-         (collect_func (Smallstep.globalenv (linked_list_sem se))
-            find_func))
-      (InitDomain.add_place_list
-         (collect_func (Smallstep.globalenv (linked_list_sem se))
-            find_func)
-         (places_of_locals (fn_params find_func ++ fn_vars find_func))
-         (PTree.map
-            (fun (_ : positive) (_ : InitDomain.LPaths.t) =>
-             InitDomain.Paths.empty)
-            (collect_func (Smallstep.globalenv (linked_list_sem se))
-               find_func)))
-      (collect_func (Smallstep.globalenv (linked_list_sem se))
-         find_func)) with true.
-
-
-native_compute (check_own_env_consistency
-      (PTree.map
-         (fun (_ : positive) (_ : InitDomain.LPaths.t) =>
-          InitDomain.Paths.empty)
-         (collect_func (proj1_sig build_ce_ok) find_func))
-      (PTree.map
-         (fun (_ : positive) (_ : InitDomain.LPaths.t) =>
-          InitDomain.Paths.empty)
-         (collect_func (proj1_sig build_ce_ok) find_func))
-      (InitDomain.add_place_list
-         (collect_func (proj1_sig build_ce_ok) find_func)
-         (places_of_locals (fn_params find_func ++ fn_vars find_func))
-         (PTree.map
-            (fun (_ : positive) (_ : InitDomain.LPaths.t) =>
-             InitDomain.Paths.empty)
-            (collect_func (proj1_sig build_ce_ok) find_func)))
-      (collect_func (proj1_sig build_ce_ok) find_func) = true).
-{ simpl
-
-
-    
-  rewrite H.
-             
-               
-        econstructor.
-        eapply find_args_params_norepet.
-        eapply do_alloc_variables_sound. simpl.
-        do 9 destruct Mem.alloc eqn: ?ALLOC at 1. f_equal.
-
-        Lemma find_step_internal_progress
+End SOUNDNESS.
 
 
         
